new/user_rc/Enable-wins_flag/App_user_rc.fst
@@ -38,18 +38,10 @@ type app_op_t:eqtype =
   |Disable
 
 // apply an operation to a state
-(*let do (s:concrete_st) (o:op_t) : concrete_st =
+let do (s:concrete_st) (o:op_t) : concrete_st =
   match o with
   |(_, (rid, Enable)) -> M.upd s rid (fst (sel s rid) + 1, true) 
-  |(_, (rid, Disable)) -> M.map_val (fun (c,f) -> (c, false)) s *)
-let do (s:concrete_st) (o:op_t) 
-  : (r:concrete_st{(Enable? (snd (snd o)) ==> sel r (get_rid o) = (fst (sel s (get_rid o)) + 1, true) /\
-                                              (forall rid. rid <> get_rid o ==> sel r rid = sel s rid)) /\
-                   (Disable? (snd (snd o)) ==> (forall rid. sel r rid = (fst (sel s rid), false)))}) =
-  match o with
-  |(_, (rid, Enable)) -> M.upd s rid (fst (sel s rid) + 1, true) 
-  |(_, (rid, Disable)) -> M.map_val (fun (c,f) -> (c, false)) s 
-
+  |(_, (rid, Disable)) -> M.map_val (fun (c,f) -> (c, false)) s
 let lem_do (a b:concrete_st) (op:op_t)
    : Lemma (requires eq a b)
            (ensures eq (do a op) (do b op)) = ()
@@ -87,16 +79,10 @@ let merge_cf (l a b:cf) : cf =
   (fst a + fst b - fst l, merge_flag l a b)
   
 // concrete merge operation
-(*let merge (l a b:concrete_st) : concrete_st =
+let merge (l a b:concrete_st) : concrete_st =
   let keys = S.union (M.domain l) (S.union (M.domain a) (M.domain b)) in
   let u = M.const_on keys (0, false) in
-  M.iter_upd (fun k v -> merge_cf (sel l k) (sel a k) (sel b k)) u*)
-let merge (lca s1 s2:concrete_st) 
-  : (r:concrete_st{(forall rid. M.contains r rid <==> M.contains lca rid \/ M.contains s1 rid \/ M.contains s2 rid) /\
-                   (forall rid. sel r rid = merge_cf (sel lca rid) (sel s1 rid) (sel s2 rid))}) =  
-  let keys = S.union (M.domain lca) (S.union (M.domain s1) (M.domain s2)) in
-  let u = M.const_on keys (0, false) in
-  M.iter_upd (fun k v -> merge_cf (sel lca k) (sel s1 k) (sel s2 k)) u
+  M.iter_upd (fun k v -> merge_cf (sel l k) (sel a k) (sel b k)) u
 
 
 /////////////////////////////////////////////////////////////////////////////
@@ -110,16 +96,36 @@ let merge_comm (l a b:st)
 let merge_idem (s:st)
   : Lemma (ensures eq (merge (v_of s) (v_of s) (v_of s)) (v_of s)) = ()
 
-let fast_fwd (a b:st)
-  : Lemma (requires cons_reps a a b)
-          (ensures eq (merge (v_of a) (v_of a) (v_of b)) (v_of b)) = admit()
+#push-options "--z3rlimit 50 --ifuel 3 --split_queries always"
+let fast_fwd_base (a b:st) (last2:op_t)
+  : Lemma (ensures eq (do (v_of a) last2) (merge (v_of a) (v_of a) (do (v_of a) last2))) = ()
 
+let rec lem_apply (x:concrete_st) (l:log)
+  : Lemma (ensures (let r = apply_log x l in
+                        (forall rid. M.contains x rid ==> M.contains r rid) /\
+                        (forall rid. fst (sel r rid) >= fst (sel x rid))))
+          (decreases length l) =
+  match length l with
+  |0 -> ()
+  |_ -> lem_apply (do x (head l)) (tail l)
+
+let fast_fwd_ind (a b:st) (last2:op_t)
+  : Lemma (requires length (ops_of b) > length (ops_of a) /\
+                    (let b' = inverse_st b in
+                    cons_reps a a b' /\
+                    eq (do (v_of b') last2) (merge (v_of a) (v_of a) (do (v_of b') last2))))
+        
+          (ensures eq (do (v_of b) last2) (merge (v_of a) (v_of a) (do (v_of b) last2))) = 
+  let b' = inverse_st b in
+  split_prefix init_st (ops_of a) (ops_of (do_st b' last2));
+  lem_apply init_st (ops_of a);
+  lem_apply (v_of a) (diff (snoc (ops_of b') last2) (ops_of a))
+  
 let merge_eq (l a b a':concrete_st)
   : Lemma (requires eq a a')
           (ensures eq (merge l a b)
                       (merge l a' b)) = ()
 
-#push-options "--z3rlimit 50 --ifuel 3"
 let lin_rc_ind_b' (l a b:st) (last1 last2:op_t)
   : Lemma (requires length (ops_of b) > length (ops_of l) /\
                     fst last1 <> fst last2 /\ ~ (comm_ops last1 last2) /\ Fst_snd? (rc last1 last2) /\
@@ -168,83 +174,36 @@ let lin_comm_ind_b' (l a b:st) (last1 last2:op_t)
           (ensures eq (do (merge (v_of l) (do (v_of a) last1) (v_of b)) last2)
                       (merge (v_of l) (do (v_of a) last1) (do (v_of b) last2))) = ()
 
-let lin_comm_ind_a'_dd (l a b:st) (last1 last2:op_t)
-  : Lemma (requires length (ops_of a) > length (ops_of l) /\
-                    comm_ops last1 last2 /\ Disable? (snd (snd last1)) /\ Disable? (snd (snd last2)) /\
+let lin_comm_ind_a' (l a b:st) (last1 last2:op_t)
+  : Lemma (requires //cons_reps l a b /\ 
+                    length (ops_of a) > length (ops_of l) /\
+                    comm_ops last1 last2 /\
+                    ops_of b = ops_of l /\
                     (let a' = inverse_st a in
                     eq (do (merge (v_of l) (do (v_of a') last1) (v_of b)) last2)
                        (merge (v_of l) (do (v_of a') last1) (do (v_of b) last2))))
                            
           (ensures eq (do (merge (v_of l) (do (v_of a) last1) (v_of b)) last2)
                       (merge (v_of l) (do (v_of a) last1) (do (v_of b) last2))) = ()
-
-let rec lem_apply (x:concrete_st) (l:log)
-  : Lemma (ensures (let r = apply_log x l in
-                        (forall rid. M.contains x rid ==> M.contains r rid) /\
-                        (forall rid. fst (sel r rid) >= fst (sel x rid))))
-          (decreases length l) =
-  match length l with
-  |0 -> ()
-  |_ -> lem_apply (do x (head l)) (tail l)
-
-let lin_comm_ind_a'_ee_help (l a b:st) (last1 last2:op_t)
-  : Lemma (requires cons_reps l a b)                           
-          (ensures (forall id. M.contains (v_of l) id ==> M.contains (do (v_of a) last1) id /\  M.contains (v_of b) id) /\
-                   (forall id. M.contains (merge (v_of l) (do (v_of a) last1) (v_of b)) id ==>
-                          fst (sel (do (v_of a) last1) id) >= fst (sel (v_of l) id) /\
-                          fst (sel (v_of b) id) >= fst (sel (v_of l) id))) = 
-  lem_apply init_st (ops_of l);  
-  split_prefix init_st (ops_of l) (ops_of b);
-  lem_apply (v_of l) (diff (ops_of b) (ops_of l));
-  split_prefix init_st (ops_of l) (ops_of (do_st a last1));
-  lem_apply (v_of l) (diff (snoc (ops_of a) last1) (ops_of l))
-
-#push-options "--z3rlimit 200 --split_queries always"
-let lin_comm_ind_a'_ee (l a b:st) (last1 last2:op_t)
-  : Lemma (requires cons_reps l a b /\
-                    length (ops_of a) > length (ops_of l) /\
-                    comm_ops last1 last2 /\ Enable? (snd (snd last1)) /\ Enable? (snd (snd last2)) /\
-                    (let a' = inverse_st a in
-                    eq (do (merge (v_of l) (do (v_of a') last1) (v_of b)) last2)
-                       (merge (v_of l) (do (v_of a') last1) (do (v_of b) last2))))
-                           
-          (ensures eq (do (merge (v_of l) (do (v_of a) last1) (v_of b)) last2)
-                      (merge (v_of l) (do (v_of a) last1) (do (v_of b) last2))) = 
-  lin_comm_ind_a'_ee_help l a b last1 last2
-
-let lin_comm_ind_a' (l a b:st) (last1 last2:op_t)
-  : Lemma (requires cons_reps l a b /\ length (ops_of a) > length (ops_of l) /\
-                    comm_ops last1 last2 /\
-                    (let a' = inverse_st a in
-                    eq (do (merge (v_of l) (do (v_of a') last1) (v_of b)) last2)
-                       (merge (v_of l) (do (v_of a') last1) (do (v_of b) last2))))
-                           
-          (ensures eq (do (merge (v_of l) (do (v_of a) last1) (v_of b)) last2)
-                      (merge (v_of l) (do (v_of a) last1) (do (v_of b) last2))) =
-  if Enable? (snd (snd last1)) && Enable? (snd (snd last2)) then 
-    lin_comm_ind_a'_ee l a b last1 last2
-  else lin_comm_ind_a'_dd l a b last1 last2
-
-#push-options "--z3rlimit 100 --split_queries always"
+                      
 let rec lin_comm1 (l a b:st) (last1 last2:op_t)
   : Lemma (requires cons_reps l a b /\
                     fst last1 <> fst last2 /\ comm_ops last1 last2)
                     //~ (reorder last2 (diff (snoc (ops_of a) last1) (ops_of l))))
           (ensures eq (do (merge (v_of l) (do (v_of a) last1) (v_of b)) last2)
                       (merge (v_of l) (do (v_of a) last1) (do (v_of b) last2)))
-          (decreases %[length (ops_of a); length (ops_of b)]) =
+          (decreases %[length (ops_of a); length (ops_of b)]) = 
   if ops_of a = ops_of l && ops_of b = ops_of l then ()
-  else if ops_of a = ops_of l then 
-    (let b' = inverse_st b in 
-     cons_reps_s2' l a b; 
-     lin_comm1 l a b' last1 last2;
-     lin_comm_ind_b' l a b last1 last2) 
-  else 
+  else if ops_of b = ops_of l then 
     (let a' = inverse_st a in
-     let _, last1' = un_snoc (ops_of a) in
      cons_reps_s1' l a b;
      lin_comm1 l a' b last1 last2;
      lin_comm_ind_a' l a b last1 last2)
+  else 
+    (let b' = inverse_st b in
+     cons_reps_s2' l a b;
+     lin_comm1 l a b' last1 last2;
+     lin_comm_ind_b' l a b last1 last2)
 #pop-options
 
 let lin_comm (l a b:st) (last1 last2:op_t)
